Binary_inter_nbhds and directed nbhds

basic_topology/T5_nets.lean
@@ -19,102 +19,56 @@ def Endorelation (X : Type u) : Type u :=
   Relation X X
 
 /-- A preorder is a reflexive and transitive relation. -/
-structure preorder (X : Type u) (R : Relation X X) : Prop where
+structure preorder {X : Type u} (R : Relation X X) : Prop where
   reflexive : ∀ x, R x x
   transitive : ∀ x y z, (R x y ∧ R y z) → R x z
 
 /-- A directed set is a preorder where any two elements have an upper bound. -/
-structure directed_set (X : Type u) (R : Relation X X) : Prop where
-  reflexive : ∀ x, R x x
-  transitive : ∀ x y z, (R x y ∧ R y z) → R x z
+structure directed_set {X : Type u} (R : Relation X X) : Prop extends preorder R where
   upperbound : ∀ x y, ∃ z, R x z ∧ R y z
 
-/-- A net in `X` is a function from a directed set into `X`. -/
-structure net (X : Type u) where
-  (D : Type v)
-  (R : Relation D D)
-  [is_directed : directed_set D R]
-  (a : D → X)
-def f_net {X Y : Type*} (f : X → Y) (n : net X) : net Y :=
-  { D := n.D,
-    R := n.R,
-    is_directed := n.is_directed,
-    a := fun i => f (n.a i) }
 
-/-- A net `n` converges to `x` with respect to the topology `𝒯`
-iff every open neighborhood of `x` eventually contains all later terms of the net. -/
-def net_converges {X : Type u} (T: Set (Set X)) (n : net X) (x : X) : Prop :=
-  ∀ U : Set X, (U ∈ T) → (x ∈ U) →
-    ∃ i₀ : n.D, ∀ j : n.D, n.R i₀ j → n.a j ∈ U
-def f_net_converges
-  {X Y : Type*}
-  (TY : Set (Set Y))
-  (f : X → Y)
-  (n : net X)
-  (y : Y) : Prop :=
-  net_converges TY (f_net f n) y
-/--
-The neighborhood net of a point `x` is a net constructed from the directed set of
-neighborhoods of `x`, where the direction is given by reverse subset inclusion.
-For each neighborhood `V`, a point `a(V)` is chosen from `V` using the axiom of choice.
--/
-noncomputable def neighborhood_net {X : Type u} (TX: Set (Set X)) (hTX : IsTopology TX) (x : X) : net X where
-  D := { V : Set X // V ∈ Nbhds TX x }
-  R := fun U V => V.1 ⊆ U.1
-  is_directed := {
-    reflexive := fun U => Set.Subset.refl U.1,
-    transitive := fun _ _ _ h => Set.Subset.trans h.2 h.1,
-    upperbound := fun U V => by
-      have h_inter_nhds : U.1 ∩ V.1 ∈ Nbhds TX x := by
-        obtain ⟨O_U, hO_U_open, hx_in_OU, hOU_sub_U⟩ := U.2
-        obtain ⟨O_V, hO_V_open, hx_in_OV, hOV_sub_V⟩ := V.2
-        use O_U ∩ O_V
-        exact ⟨binary_inter_open hTX hO_U_open hO_V_open, ⟨hx_in_OU, hx_in_OV⟩, Set.inter_subset_inter hOU_sub_U hOV_sub_V⟩
-      use ⟨U.1 ∩ V.1, h_inter_nhds⟩
-      exact ⟨Set.inter_subset_left, Set.inter_subset_right⟩
-  }
-  a := fun V => Classical.choose (Set.nonempty_of_mem (neighborhood_mem V.2))
+def net_converges {X : Type u} {D : Type v} (T: Set (Set X)) (R: Relation D D) (a: D -> X) (x: X) : Prop :=
+  ∀ U ∈ Nbhds T x, ∃ i₀, ∀ j, R i₀ j → a j ∈ U
 
-/-- The neighborhood net of a point `x` converges to `x`. -/
-theorem neighborhood_net_converges {X : Type u} (TX: Set (Set X)) (hTX : IsTopology TX) (x : X) :
-  net_converges TX (neighborhood_net TX hTX x) x := by
-  rw [net_converges]
-  intro U hU_open hx_in_U
-  use ⟨U, open_neighborhood TX hx_in_U hU_open⟩
-  rintro ⟨A, hA⟩ hA_sub_U
-  have point_in_A := Classical.choose_spec (Set.nonempty_of_mem (neighborhood_mem hA))
-  exact hA_sub_U point_in_A
+-- A helper for the image of a net.
+def f_net_converges {X Y : Type u} {D : Type v} (TY: Set (Set Y)) (R: Relation D D) (f: X -> Y) (a: D -> X) (y: Y) : Prop :=
+  net_converges TY R (f ∘ a) y
 
+def neighborhood_direction (T: Set (Set X)) (x: X): Endorelation (Nbhds T x) :=
+  fun N1 N2 => N2.1 ⊆ N1.1
 
+theorem neighborhood_direction_directed_set (T: Set (Set X)) (x: X) (hT: IsTopology T) : (directed_set (neighborhood_direction T x)) := by
+  repeat constructor
+  intro Nx
+  exact fun ⦃a⦄ a ↦ a
+  simp [neighborhood_direction]
+  intro N1 hN1 N2 hN2 N3 hN3
+  exact fun a a_1 ⦃a_2⦄ a_3 ↦ a (a_1 a_3)
+  intro ⟨N1,hN1⟩ ⟨N2,hN2⟩
+  simp [neighborhood_direction]
+  use N1∩N2
+  repeat constructor
+  exact Set.inter_subset_left
+  constructor
+  exact neighborhood_binary_inter x N1 hT N2 hN1 hN2
+  exact Set.inter_subset_right
 
-
-theorem continuous_at_iff_f_net_converges
-  {X Y : Type*} (TX: Set (Set X))(TY: Set (Set Y))
-  (hTX : IsTopology TX) (hTY : IsTopology TY)
-  (f : X → Y) (x0 : X) :
-  continuous_at TX TY f x0 ↔
-    ∀ n : net X, net_converges TX n x0 → f_net_converges TY f n (f x0):= by
+theorem continuous_at_iff_all_nets_converge {X: Type u} {TX: Set ( Set X)} {TY: Set (Set Y )} (hTX: IsTopology TX ) (hTY: IsTopology TY) (f:X→ Y) (x0:X):
+  continuous_at TX TY f x0 ↔ ∀D : Type u , ∀ R: Endorelation D , directed_set R → ∀ x: D → X , net_converges TX R x x0 → net_converges TY R (f∘ x) (f x0):= by
     constructor
-    intro h n hn
-    rw[continuous_at] at h
-    simp[f_net_converges,net_converges]
-    intro U hU hf
-    have h1 : U∈ Nbhds TY (f x0) := by
-      simp [Nbhds]
-      exact open_neighborhood TY hf hU
-    apply h at h1
-    obtain ⟨ N,hN⟩ := h1
-    simp [f_net]
-    simp[net_converges] at hn
-    simp [Nbhds,neighborhood] at hN
-    obtain ⟨ O,hO⟩ := hN.left
-    let h3:= hO.left
-    apply hn at h3
-    have h4: x0∈ O:= by exact hO.right.left
-    apply h3 at h4
-    obtain ⟨ i,hi⟩ := h4
+    simp[net_converges]
+    intro h_con D  R  d  hR hnx
+    rw[continuous_at] at h_con
+    intro U hU
+    apply h_con at hU
+    obtain ⟨ N, ⟨ hN1,hN2⟩ ⟩ := hU
+    apply hnx at hN1
+    obtain ⟨ i,hi⟩ := hN1
     use i
-    intro j hj
-    exact hN.2 (hO.2.2 (hi j hj))
-    intro hn N hN
-    sorry
+    intro j hrij
+    apply hN2
+    exact Set.mem_image_of_mem f (hi j hrij)
+    contrapose
+    push_neg
+    intro h_con
